\documentclass{article}

\begin{document}

\begin{enumerate}
\item
\[
\frac{\partial \log p(x_{t+1}|x_{1:t})}{\partial \alpha} = \frac{1}{p(x_{t+1}|x_{1:t})} \sum_{r_{t}} p(x_{t+1}|r_{t},x_{t-r_{t}:t}) p(r_{t}|x_{1:t}) \frac{\partial \log p(r_{t}|x_{1:t})}{\partial \alpha}
\]
\item
\[
\frac{\partial \log p(r_{t}|x_{1:t})}{\partial \alpha} = \frac{1}{p(r_{t},x_{1:t})} - \frac{\partial \log p(x_{1:t})}{\partial \alpha}
\]
where 
\[
\frac{\partial \log p(x_{1:t})}{\partial \alpha} = \frac{1}{p(r_{t},x_{1:t})} \sum_{r_{t}} p(r_{t},x_{1:t}) \frac{\partial \log p(r_{t},x_{1:t})}{\partial \alpha}
\]
\item
\[
\frac{\partial \log p(r_{t}=r_{t-1}+1,x_{1:t})}{\partial \alpha} = \frac{\partial \log p(r_{t}=r_{t-1}+1|r_{t-1},\alpha)}{\partial \alpha} + \frac{\partial \log p(r_{t-1},x_{1:t-1})}{\partial \alpha}
\]
\[
\frac{\partial \log p(r_{t}=0,x_{1:t})}{\partial \alpha} = A/B
\]
where
\[
A = \sum_{r_{t-1}} p(r_{t}=0|r_{t-1},\alpha)p_{prior}(x_{t})p(r_{t-1},x_{1:t-1})\left[\frac{\partial \log p(r_{t}=0|r_{t-1},\alpha)}{\partial \alpha} + \frac{\partial \log p(r_{t-1},x_{1:t-1})}{\partial \alpha} \right]
\]
and
\[
B = \sum_{r_{t-1}} p(r_{t}=0|r_{t-1},\alpha)p_{prior}(x_{t})p(r_{t-1},x_{1:t-1})
\]
\end{enumerate}

\end{document}